Logics are able to derive type class instances for function spaces.

MirrorCharge!/src/ILPullQuant.v
@@ -1,4 +1,9 @@
-Require Import ILogic ILogicFunc.
+Add Rec LoadPath "/Users/jebe/git/Charge/Charge!/bin".
+Add Rec LoadPath "/Users/jebe/git/mirror-core/src/" as MirrorCore.
+Add Rec LoadPath "/Users/jebe/git/mirror-core/coq-ext-lib/theories" as ExtLib.
+Add Rec LoadPath "/Users/jebe/git/MirrorCharge/MirrorCharge!/bin".
+
+Require Import ILogic ILInsts ILogicFunc.
 Require Import MirrorCore.Ext.Types.
 Require Import MirrorCore.Ext.ExprCore.
 Require Import MapPositive.
@@ -8,28 +13,610 @@ Require Import Coq.Bool.Bool.
 Require Import ExtLib.Data.Positive.
 Require Import Ext.ExprLift.
 Require Import ExtLib.Tactics.Consider.
+Require Import MirrorCore.Ext.Expr.
 Require Import MirrorCore.Ext.ExprD.
 Require Import MirrorCore.Ext.ExprTactics.
+Require Import MirrorCore.EnvI.
 Require Import ExtLib.Tactics.Cases.
 Require Import ExtLib.Tactics.Injection.
 Require Import ExtLib.Tactics.EqDep.
+Require Import Ext.SetoidFold.
+Require Import Relation_Definitions.
 
 Set Implicit Arguments. 
 Unset Strict Implicit.
 Set Maximal Implicit Insertion.
 
-Definition inhabited (ts : types) := forall (t : typ),
+Definition inhabited (ts : types)  := forall (t : typ),
   option (Inhabited (typD ts nil t)).
+  
+Section Relation.
+	Variable ts : types.
+	Variable func : Type.
+	Variable R : RSym (typD ts) func.
+	Variable us vs : tenv typ.
+
+	Definition is_relation_bool (t : typ) := 
+		match t with 
+			| tyArr t (tyArr t' tyProp) => t ?[eq] t'
+			| _                          => false
+		end. 
+
+	Definition is_relation (e : expr func) (t : typ) :=
+		WellTyped_expr us vs e (tyArr t (tyArr t tyProp)).
+		
+End Relation.
+ 
+Section IsPreOrder.
+	Variable ts : types.
+	Variable func : Type.
+	Variable us vs : env (typD ts).
+	Variable R : RSym (typD ts) func.
+
+	Variable is_preorder : expr func -> bool.
+	
+	Definition preorder_prop (e : expr func) (t : typ) := 
+		forall v, exprD us vs e (tyArr t (tyArr t tyProp)) = Some v ->
+		PreOrder v.
+
+	Definition is_preorder_sound :=
+	    forall e, is_preorder e = true -> forall t, preorder_prop e t.
+
+End IsPreOrder.
 
 Section PullExistsLeft.
   Context (ts : types) (funcs : fun_map ts) (gs : logic_ops ts).
-  Context (H : forall g, match gs g with
-                             | Some T => @ILogic _ T
-                             | None => unit
-                           end).
-                           
-  Local Instance RSym_ilfunc : SymI.RSym (typD ts) ilfunc := RSym_ilfunc ts funcs gs.
 
+  Local Instance RSym_sym : SymI.RSym (typD ts) ilfunc := RSym_ilfunc ts funcs gs.
+
+  Variable us vs : env (typD ts).                       
+  Definition T := (list type * list typ * expr ilfunc)%type.
+
+  Definition T_union (p q : T) : T :=
+  	(fst (fst p) ++ fst (fst q), snd (fst p) ++ snd (fst q),
+         App (lift 0 (length (fst (fst q))) (snd p)) (snd q)).
+
+  Definition T_to_expr (t : T) (il : typ) := 
+    fold_right (fun t e => App (Inj (ilf_exists t il)) (Abs t e)) (snd t) (fst t).
+
+  Inductive Rbase := 
+    | Ent t : (exists v, gs' ts gs t = Some v) -> Rbase
+    | Eq : Rbase.
+
+  Fixpoint Rbase_eq (r1 r2 : Rbase) : bool :=
+    match r1, r2 with
+      | Ent t1 _, Ent t2 _ => t1 ?[eq] t2
+      | Eq, Eq             => true
+      | _, _               => false
+    end.
+
+  Instance RelDec_Rbase_eq : RelDec (@eq Rbase) := { rel_dec := Rbase_eq }.
+
+  Definition typeForRbase r := 
+    match r with 
+      | Ent t _ => t
+      | Eq => tyProp
+    end.
+
+  Definition app (vs us : tenv typ) (pq p : T) (rpq rp : R Rbase) : option T := 
+    match rpq with
+      | Rinj (Ent t _) =>
+        Some (fst pq ++ fst p, App (lift 0 (length (fst p)) (snd pq)) (snd p))
+      | Rpointwise t (Ent t' _) => 
+      | _ => None
+    end.
+
+  Definition abs (vs us : tenv typ) (t : typ) (p : T) (r : R Rbase) : option T :=
+    Some (t :: fst p, snd p).
+
+  Fixpoint unify (r : R Rbase) (p : PR Rbase) : bool :=
+    match p with
+      | PRguess => true
+      | PRinj i => match r with
+                     | Rinj i' => i ?[ eq ] i'
+                     | _ => false
+                   end
+      | PRfunctorial a b =>
+        match r with
+          | Rfunctorial a' b' => andb (unify a' a) (unify b' b)
+          | _ => false
+        end
+      | PRpointwise t a =>
+        match r with
+          | Rpointwise t' a' => andb (t ?[eq] t') (unify a' a)
+          | _ => false
+        end
+    end.
+
+  Definition proper_lookup (a : expr ilfunc)  (r : Rbase) : option (R Rbase) :=
+    match a, r with
+      | Inj (ilf_and t), Ent t' pr => 
+        if t ?[eq] t' then  
+          Some (Rfunctorial (Rinj (Ent pr)) ((Rfunctorial (Rinj (Ent pr)) (Rinj (Ent pr)))))
+        else
+          None
+      | Inj (ilf_exists a t), Ent t' pr =>
+        if t ?[eq] t' then
+          Some (Rfunctorial (Rpointwise a (Rinj (Ent pr))) (Rinj (Ent pr)))
+        else
+          None
+      | Inj (ilf_true t), Ent t' pr => if t ?[eq] t' then Some (Rinj (Ent pr)) else None
+(*      | _, Ent (tyType 0) pr => match @typeof_expr (@ILogicFunc.ts A) ilfunc (RSym_sym funcs logics) nil nil a with
+                               | Some (tyType 0) => Some (Rinj (Ent pr))
+                               | _ => None
+                                end*)
+      | _, _ => None
+    end.
+
+
+
+  Fixpoint get_proper_aux (e : expr ilfunc) (r : PR Rbase) : option (R Rbase) :=
+    match r with
+      | PRinj r => proper_lookup e r
+      | PRfunctorial l r => get_proper_aux e r 
+      | PRpointwise t r => get_proper_aux e r
+      | _ => None
+    end.
+
+  Definition get_unified_proper (e : expr ilfunc) (r : PR Rbase) : option (R Rbase) := 
+    match get_proper_aux e r with
+      | Some x => if unify x r then Some x else None
+      | None => None
+    end.
+
+  Lemma unification_instantiates r r' (H : unify r' r = true) :
+    instantiates r' r.
+  Proof.
+    
+    generalize dependent r; induction r'; simpl; intros.
+    + destruct r0; try congruence; [|apply Ins_guess]. admit.
+    + destruct r; try congruence; [apply Ins_guess|].
+      rewrite andb_true_iff in H. apply Ins_func; [apply IHr'1| apply IHr'2]; intuition.
+    + destruct r; try congruence; [apply Ins_guess|].
+      rewrite andb_true_iff in H.
+      assert (t = t0) by admit; subst.
+      apply Ins_point. apply IHr'; intuition.
+  Qed.
+
+  Definition atom (us vs : tenv typ) (e : expr ilfunc) (r : R Rbase) : option T := Some (nil, e).
+
+  Definition TD us vs (t : T) (il : typ) := exprD us vs (T_to_expr t il) il.
+
+  Fixpoint RD (r : R Rbase) : (typD ts nil (typeForR typeForRbase r)) -> 
+                              (typD ts nil (typeForR typeForRbase r)) -> Prop :=
+    match r with
+      | Rfunctorial l r => fun f g => forall x y, @RD l x y -> @RD r (f x) (g y)
+      | Rinj (Ent t _) => 
+        fun a b => t ?[eq] typeForR typeForRbase r = true /\
+                   exists ILO, gs' ts gs t = Some ILO /\ a |-- b
+      | Rinj Eq => fun a b => a = b
+      | Rpointwise t r => fun f g => forall x, @RD r (f x) (g x)
+    end.
+
+  Lemma RD_reflexive r a : @RD r a a.
+  Proof.
+    induction r.
+    + simpl. destruct r; [|reflexivity].
+      split. simpl. apply rel_dec_eq_true. apply _. reflexivity.
+      destruct e. simpl in *.
+      exists x. intuition. admit.
+    + simpl; intros.
+      admit. (* This is not true *)
+    + simpl; intros.
+      apply IHr.
+  Qed.
+
+  Definition TR us vs (r : R Rbase) (t : T) v : Prop :=
+    exists v', TD us vs t (typeForR typeForRbase r) = Some v' /\ @RD r v v'.
+(*
+  Theorem Hatomic
+    : forall tus tvs e r r' result,
+        get_unified_proper  e r = Some r' ->
+        (atom tus tvs e r' = Some result) ->
+        @setoid_fold_spec _ _ (RSym_sym) _ _ _ TR tus tvs e r result r'.
+  Proof.
+    intros; repeat split; intros.
+    + apply unification_instantiates.
+      unfold get_unified_proper in H.
+      destruct (get_proper_aux e r); try congruence.
+      remember (unify r0 r) as b; destruct b; congruence.
+    + unfold get_unified_proper in H.
+      remember (get_proper_aux e r) as o; destruct o; try congruence.
+      remember (unify r0 r) as b; destruct b; try congruence.
+      inv_all; subst.
+      clear H1; clear Heqb.
+      generalize dependent r'.
+      induction r; intros; simpl in *.
+      
+      
+  Lemma unification_type r r' t (H : unify r' r = true) 
+    (H1 : pr_type typeForRbase r t) : typeForR typeForRbase r' = t.
+  Proof.
+    generalize dependent r; induction r'; simpl; intros.
+    + destruct r0; try congruence.
+      - assert (r0 = r) by admit; subst. 
+        inversion H1; reflexivity.
+      - 
+  Qed.
+ 
+Print pr_type.
+    + remember (exprD' us0 tvs e (typeForR typeForRbase r')).
+      destruct o; [|apply I].
+      intros. unfold atom in H0. inversion H0; subst.
+      unfold TR.
+      clear H0. exists (t0 vs0).
+      split. unfold TD. simpl.
+      unfold exprD; simpl.
+      rewrite split_env_join_env.
+      unfold T_to_expr; simpl.
+      remember (exprD' us0 tvs e (typeForR typeForRbase r')).
+      destruct o; inv_all; subst; [reflexivity|congruence].
+      apply RD_reflexive.
+  Qed.
+*)
+  Definition SRW_Algo_pull_quant := 
+    @SRW_Algo_properAt ilfunc T Rbase get_unified_proper atom app abs.
+                                                       
+End PullExistsLeft.
+
+Section demo.
+  Context {A : Type} {ILO : ILogicOps A}.
+
+  Context (logics_sound : forall g, match logics g with
+                                  | Some T => @ILogic _ T
+                                  | None => unit
+                                end).
+
+  Existing Instance ILFun_ILogic.
+  
+  Lemma gs'_sound : forall g, match gs' ts logics g with 
+                                | Some T => @ILogic _ T
+                                | None => unit
+                              end.
+  Proof.
+    intros g; induction g; simpl; try apply tt.
+    simpl. remember (gs' ts logics g2) as o; destruct o; [apply _ | apply tt].
+    destruct n; [|apply tt]; simpl in *.
+    specialize (logics_sound (tyType 0)); simpl in *.
+    apply logics_sound.
+  Qed.
+
+  Program Definition ent := @Ent _ logics (tyType 0) _.
+  Next Obligation.
+    exists ILO. reflexivity.
+  Defined.
+
+Print setoid_fold_spec.
+(*
+Check @exprD'.
+Print setoid_fold_spec.
+  Definition TR us vs (r : R (Rbase logics)) (t : T) v : Prop :=
+    exists v', TD us vs t (typeForR typeForRbase r) = Some v' /\ @RD us vs r v v'.
+
+
+  Theorem Hatomic
+    : forall tus tvs e r r' result,
+        (get_unified_proper get_proper)  e r = Some r' ->
+        (atom tus tvs e r' = Some result) ->
+        @setoid_fold_spec _ _ (RSym_sym funcs logics) _ _ _ TR tus tvs e r result r'.
+  Proof.
+    intros.
+    unfold atom in H0. inv_all; subst.
+    red; intros.
+    split. admit.
+    split. admit.
+    intros.
+    remember (exprD' us tvs e (typeForR typeForRbase r')) as o.
+    destruct o; [|apply I]. 
+    intros.
+    unfold TR. exists (t0 vs).
+    split.
+    unfold TD.
+    unfold exprD.
+    simpl.
+    simpl.
+    
+    
+
+  
+
+  Check SRW_AlgoOk_properAt.
+*)
+  Eval compute in
+      @setoid_fold _ _ _ (atomic (SRW_Algo_pull_quant logics)) (SetoidFold.app (SRW_Algo_pull_quant logics))
+                   (SetoidFold.abs (SRW_Algo_pull_quant logics)) nil nil
+                   inj_true
+                   (Rinj ent).
+
+  Eval compute in
+      @setoid_fold _ _ _ (atomic (SRW_Algo_pull_quant logics)) (SetoidFold.app (SRW_Algo_pull_quant logics))
+                   (SetoidFold.abs (SRW_Algo_pull_quant logics)) nil nil
+                   (inj_and inj_true inj_true)
+                   (Rinj ent).
+
+  Eval compute in
+      @setoid_fold _ _ _ (atomic (SRW_Algo_pull_quant logics)) (SetoidFold.app (SRW_Algo_pull_quant logics))
+                   (SetoidFold.abs (SRW_Algo_pull_quant logics)) nil nil
+                   (inj_exists (tyType 1) inj_true)
+                   (Rinj ent).
+
+Definition test_fold := @setoid_fold _ _ _ (atomic (SRW_Algo_pull_quant logics)) (SetoidFold.app (SRW_Algo_pull_quant logics))
+                   (SetoidFold.abs (SRW_Algo_pull_quant logics)) nil nil.
+
+Eval compute in test_fold (Abs (tyType 1) inj_true) (Rpointwise (tyType 1) (Rinj ent)).
+Eval compute in test_fold (Inj (ilf_exists (tyType 1) (tyType 0))) (Rfunctorial (Rpointwise (tyType 1) (Rinj ent)) (Rinj ent)).
+
+
+
+Eval compute in 
+  Eval compute in
+      @setoid_fold _ _ _ (atomic SRW_Algo_pull_quant) (SetoidFold.app SRW_Algo_pull_quant)
+                   (SetoidFold.abs SRW_Algo_pull_quant) nil nil 
+                   (inj_and (inj_exists (tyType 1) (inj_eq_nat (Var 0) (Var 0))) inj_true) 
+                   (Rinj ent).
+  simpl.
+Check @setoid_fold.
+  Eval compute in
+      @setoid_fold _ _ _ _ _ properAt atomic app nil (Inj And) (tyProp :: nil)
+                      (PRfunctorial (PRguess _ tyProp) (PRfunctorial (PRguess _ tyProp) (PRinj Impl))).
+
+  
+Check @SRW_Algo_properAt.
+  
+  Check inj_true.
+
+Check @inj_true.
+
+  Axiom eq_nat : nat -> nat -> T.
+  
+  Definition eq_nat_emb := F ts (tyArr (tyType 1) (tyArr (tyType 1) (tyType 0))) (eq_nat).
+
+  Definition inj_and (p q : expr ilfunc) : expr ilfunc := App (App (Inj (ilf_and (tyType 0))) p) q.
+
+  Lemma
+
+  Definition inj_true : expr ilfunc := Inj (ilf_true (tyType 0)).
+  Definition inj_false : expr ilfunc := Inj (ilf_false (tyType 0)).
+  Definition inj_exists (a : typ) (f : expr ilfunc) : expr ilfunc := 
+  	App (Inj (ilf_exists a (tyType 0))) (Abs a f).
+  Definition inj_forall (a : typ) (f : expr ilfunc) : expr ilfunc := 
+  	App (Inj (ilf_forall a (tyType 0))) (Abs a f).
+  Definition inj_eq_nat (a b : expr ilfunc) : expr ilfunc :=
+    App (App (Inj (fref (1%positive))) a) b.
+
+
+
+  Definition tm : expr ilfunc := inj_and inj_true inj_true.
+  Definition tm2 : expr ilfunc := inj_forall (tyType 1) (inj_eq_nat (Var 0) (Var 0)).
+  Require Import MirrorCore.Ext.ExprD.
+
+  (** TODO: Here we run into a problem because the [expr] type is
+   ** fixed to the [typ] defined in [MirrorCore.Ext.Types].
+   ** - To solve this problem, we need to abstract [expr] with respect to
+   **   types.
+   **)
+
+  Eval cbv beta iota zeta delta - [ltrue land] in @exprD ts _ (RSym_ilfunc ts funcs logics) nil nil tm (tyType 0).
+  Eval cbv beta iota zeta delta - [ltrue land lforall] in @exprD ts _ (RSym_ilfunc ts funcs logics) nil nil tm2 (tyType 0).
+
+  Check setoid_fold.
+
+End demo.
+
+
+  
+  Lemma T_to_expr_app pq p tpq tp vp vpq r
+  	(Hpq : TD pq (tyArr tp tpq) = Some vpq)
+  	(Hp : TD p tp = Some vp) :
+  	TD (app pq p r r) tpq = Some (vpq vp).
+    clear gs_sound. 
+    Set Printing All.
+clear gs.
+
+
+
+
+
+  Definition T_to_expr (t : T) (il : typ) : expr ilfunc :=
+    fold_right Abs (fold_right (fun t e => App (Inj (ilf_exists t il)) 
+                                               (Abs t e)) (snd t) (snd (fst t)))
+               (fst (fst t)).
+
+  Definition T_app (p q : T) : option T :=
+    match p, q with
+      | (l::vp, tp, ep), (nil, tq, eq) =>
+        Some (vp, tp ++ tq, App (lift 0 (length tq)  ep) eq)
+      | _, _ => None
+    end.
+
+  
+
+
+  	  
+  Definition Rbase := (typ * expr ilfunc)%type.
+
+  Definition typeForRbase (r : Rbase) : typ := fst r.
+
+  Definition app (p q : T) : T := T_union p q.
+
+  
+
+  Definition T := (list typ * list typ * expr ilfunc)%type.
+
+  Definition T_to_expr (t : T) (il : typ) : expr ilfunc :=
+    fold_right Abs (fold_right (fun t e => App (Inj (ilf_exists t il)) 
+                                               (Abs t e)) (snd t) (snd (fst t)))
+               (fst (fst t)).
+
+  Definition T_app (p q : T) : option T :=
+    match p, q with
+      | (l::vp, tp, ep), (nil, tq, eq) =>
+        Some (vp, tp ++ tq, App (lift 0 (length tq)  ep) eq)
+      | _, _ => None
+    end.
+
+  
+  	  
+  Definition T_union (p q : T) : T :=
+  	(fst p ++ fst q, App (lift 0 (length (fst q)) (snd p)) (snd q)).
+  	
+  Definition Rbase := (typ * expr ilfunc)%type.
+
+  Definition typeForRbase (r : Rbase) : typ := fst r.
+
+  Definition app (p q : T) : T := T_union p q.
+
+  
+
+
+   Fixpoint RD (r : R Rbase) : (typD ts nil (typeForR typeForRbase r)) -> 
+   (typD ts nil (typeForR typeForRbase r)) -> Prop :=
+  	match r with
+  		| Rfunctorial l r => fun f g => forall x y, @RD l x y -> @RD r (f x) (g y)
+  		| Rinj t => fun a b => exists v, exprD us vs (snd t) (tyArr (fst t) (tyArr (fst t) tyProp)) = Some v /\ v a b
+  		| Rpointwise t r => fun f g => forall x, @RD r (f x) (g x)
+  	end.
+(*
+  Lemma RD_refl (r : R Rbase) a : @RD r a a.
+  Proof.
+  	induction r.
+  	+ simpl. 
+  	  Require Import FunctionalExtensionality. 
+  	  apply functional_extensionality.
+  	destruct a.
+  	induction a.
+.*)
+  Lemma T_to_expr_app_wt p q tpq tq 
+  	(Hp : WellTyped_expr (typeof_env us) (typeof_env vs) (T_to_expr p (tyArr tq tpq)) (tyArr tq tpq))
+  	(Hq : WellTyped_expr (typeof_env us) (typeof_env vs) (T_to_expr q tq) tq) :
+  	WellTyped_expr (typeof_env us) (typeof_env vs) (T_to_expr (app p q) tpq) tpq.
+  Proof.
+  	admit.
+  Qed.
+
+  Lemma T_to_expr_app pq p tpq tp vp vpq 
+  	(Hpq : exprD us vs (T_to_expr pq (tyArr tp tpq)) (tyArr tp tpq) = Some vpq)
+  	(Hp : exprD us vs (T_to_expr p tp) tp = Some vp) :
+  	exprD us vs (T_to_expr (app pq p) tpq) tpq = Some (vpq vp).
+  Proof.
+  	unfold T_to_expr in *; simpl in *.
+  	rewrite fold_right_app.
+  	destruct p as [vps p], pq as [vpqs pq]; simpl in *. 
+  	induction vps; simpl in *. 
+  	SearchAbout exprD lift.
+  	+ generalize dependent vs. clear vs. induction vpqs; simpl in *; intros.
+  	  * rewrite exprD_App.
+  	    assert (typeof_expr (typeof_env us) (typeof_env vs) pq = Some (tyArr tp tpq)) by admit.
+  	    rewrite H0. rewrite Hpq. rewrite Hp.
+  	    rewrite typ_cast_typ_refl. reflexivity.
+  	  * simpl in *.
+  	    red_exprD. forward; subst; inv_all; revert Hpq; subst; intros.
+  	    assert (exists ILTemp, gs tpq = Some ILTemp) by admit.
+  	    destruct H0. rewrite H0.
+  	    red_exprD. forward. inv_all; subst.
+  	    rewrite typ_cast_typ_refl.
+  	    rewrite typ_cast_typ_refl.
+  	    SearchAbout exprD Abs.
+  	    unfold exprD. simpl.
+  	    destruct vs; simpl in *.
+  	    rewrite exprD'_Abs. rewrite typ_cast_typ_refl.
+  	    assert (va : typD ts nil a). admit.
+  	    
+  	    specialize (IHvpqs (fun typD => (existT (typD ts nil) a va)::nil)).
+  	    specialize (IHvpqs (a::nil)).
+  	    Print sigT.
+  	    Check HList.Hnil (typD ts nil).
+  	    specialize (IHvpqs HList.Hnil).
+  	    Print env.
+  	    unfold exprD in IHvpqs. simpl in *.
+  	    SearchAbout env.
+  	    Check @HList.Hnil.
+  	    Check @join_env.
+  	    specialize (IHvpqs (@join_env _ _ (a::nil) (HList.Hnil))).
+  	    rewrite IHvpqs.
+  	    SearchAbout Abs exprD.
+  	    Print Ltac red_exprD.
+  	    SearchAbout Abs.
+  	    Print exprD_rw.
+  	    autorewrite with exprD_rw.
+  	    rewrite exprD_Abs_is_arr.
+  	    simpl in x2.
+  	    red_exprD.
+  	    SearchAbout exprD Inj.
+  	    Print expr.
+  	    rewrite exprD_Inj.
+  	    red_exprD.
+  	    generalize dependent gs. 
+  	  Check exprD_Abs.
+  	  SearchAbout exprD Abs.
+  	  rewrite exprD_Abs.
+  	    simpl.
+  	  SearchAbout typ_cast_typ.
+  	  rewrite typeof_expr_exprD_same_type.
+  	  SearchAbout exprD typeof_expr.
+SearchAbout exprD App.
+  	 apply Hp.
+  Qed.
+  
+  Definition TR (us vs : env (typD ts)) (r : R Rbase) (t : T) v: Prop :=
+  exists v',
+    exprD us vs (T_to_expr t (typeForR typeForRbase r)) (typeForR typeForRbase r) = Some v' /\ 
+    @RD r v v'.
+  
+Lemma typeof_expr_exprDR (e : expr ilfunc) (t : typ) v
+     (Hexpr : exprD us vs e t = Some v) :   
+     WellTyped_expr (typeof_env us) (typeof_env vs) e t.
+Proof.
+	apply typeof_expr_exprD. exists v. apply Hexpr.
+Qed.
+    
+  Lemma Happ : forall t1 t2 r1 r2 v1 f,
+  exprD us vs f (typeForR typeForRbase (Rfunctorial t1 t2)) = Some v1 ->
+       @TR us vs (Rfunctorial t1 t2) r1 ->
+       @TR us vs t1 r2 ->
+       @TR us vs t2 (app r1 r2).
+  Proof.
+  	intros t1 t2 r1 r2 f v1 Hexpr [v2 [H1expr H1RD]] [v3 [H2expr H2RD]].
+	simpl in H1RD.
+	specialize (H1RD _ _ H2RD).
+	exists (v2 v3). split; [|apply H1RD].  
+	apply T_to_expr_app. assumption. assumption.
+	rewrite <- H2expr.
+	apply H2expr.	
+	simpl.
+  	apply typeof_expr_exprDR in H1expr.
+  	apply typeof_expr_exprDR in H2expr.
+  	pose proof (T_to_expr_app_wt H1expr H2expr) as Hexpr3.
+  	apply typeof_expr_exprD in Hexpr3. destruct Hexpr3 as [v Hexpr3].
+  	exists v. split. apply Hexpr3.
+	simpl in H1RD.
+	specialize (H1RD _ _ H2RD).
+	Lemma exprD_RD_app e1 e2 e12 t12 t1 t2 v12 v1 v2 v12' v1'
+	    (H12 : exprD us vs (T_to_expr e12 t12) (typeForR typeForRbase (Rfunctorial t1 t2)) = Some v12) 
+		(HRD12 : @RD (Rfunctorial t1 t2) v12 v12')
+		(HRD1 : @RD t1 v1 v1')
+	    (H1 : exprD us vs (T_to_expr e1 (typeForR typeForRbase t1)) (typeForR typeForRbase t1) = Some v1)
+		(H2 : exprD us vs (T_to_expr (app e1 e2) (typeForR typeForRbase t2)) (typeForR typeForRbase t2) = Some v2) :
+		@RD t2 (v12 v1) v2.
+	  	
+  	generalize dependent v'1.
+  	
+  	exists vpq.
+  	split. apply H3.
+  	eexists. split. apply H3.
+
+    Lemma RD_functorial t1 t2 r1 r2 f g
+    	(H1 : @RD (Rfunctorial t1 t2) r2) (Hr2 : r2 f g) (H2 : @RD t1 r1) : 
+    	@RD t2 (fun a b => forall x y, r1 x y -> a = (f x) /\ b = (g y)).
+    Proof.
+    	eapply H1. eassumption.
+    	specialize (H1 (fun a b => forall x y, r1 x y -> a = (f x) /\ b = (g y)) f g Hr2).
+   	    apply H1. simpl. in
+  	eexists.
+  	
+  	
+  	
+ 
   Fixpoint pull_exists_left (p : expr ilfunc) : (list typ * expr ilfunc) := 
   	match p with
   	  | App (App (Inj (ilf_and t)) p) q => 
